Expand bpf helper specs

lib/BPFStar.Helpers.fst
@@ -1,23 +1,60 @@
 (* BPFStar.Helpers -- implementation.
-
    All helpers are axiomatised since they are opaque BPF VM
    operations. The real implementations come from bpf_helpers.h
    at link time. *)
 module BPFStar.Helpers
 
 open Pulse.Lib.Pervasives
+module A = Pulse.Lib.Array
 open FStar.Ghost
 open BPFStar.Types
+open BPFStar.ProgType
+open BPFStar.KPtr
 
+(* Universal *)
 let bpf_get_current_pid_tgid () = admit ()
 let bpf_get_current_uid_gid () = admit ()
-let bpf_ktime_get_boot_ns () = admit ()
+let bpf_get_current_comm _ _ = admit ()
+let bpf_get_current_task () = admit ()
+let bpf_get_current_task_btf () = admit ()
+let bpf_get_ns_current_pid_tgid #_ _ _ _ _ = admit ()
+let bpf_send_signal _ = admit ()
+let bpf_send_signal_thread _ = admit ()
 let bpf_get_smp_processor_id () = admit ()
 let bpf_get_prandom_u32 () = admit ()
 
+let bpf_ktime_get_ns () = admit ()
+let bpf_ktime_get_boot_ns () = admit ()
+let bpf_ktime_get_coarse_ns () = admit ()
+let bpf_ktime_get_tai_ns () = admit ()
+let bpf_jiffies64 () = admit ()
+
 let bpf_probe_read_kernel #_ _ _ _ #_ = admit ()
 let bpf_probe_read_user #_ _ _ _ #_ = admit ()
-let bpf_probe_read_kernel_str #_ _ _ _ #_ = admit ()
-let bpf_get_current_comm #_ _ _ #_ = admit ()
+let bpf_probe_read_kernel_str _ _ _ = admit ()
+let bpf_probe_read_user_str _ _ _ = admit ()
+let bpf_copy_from_user #_ _ _ _ #_ = admit ()
 
-let bpf_printk _ = admit ()
+let bpf_trace_printk _ = admit ()
+let bpf_tail_call _ _ _ = admit ()
+
+(* Tracing family *)
+let bpf_probe_read #_ #_ #_ _ _ _ #_ = admit ()
+let bpf_probe_read_str #_ #_ _ _ _ = admit ()
+let bpf_probe_write_user #_ #_ #_ _ _ _ #_ = admit ()
+let bpf_get_stack #_ #_ _ _ _ _ = admit ()
+let bpf_get_stackid #_ #_ _ _ _ = admit ()
+let bpf_get_attach_cookie #_ #_ _ = admit ()
+
+(* Advanced tracing *)
+let bpf_d_path #_ #_ _ _ _ = admit ()
+
+(* Kprobe + fentry/fexit *)
+let bpf_get_func_ip #_ #_ _ = admit ()
+
+(* Kprobe only *)
+let bpf_override_return #_ #_ _ _ = admit ()
+
+(* LSM only *)
+let bpf_ima_inode_hash #_ #_ _ _ _ = admit ()
+let bpf_ima_file_hash #_ #_ _ _ _ = admit ()
