lib/BPFStar.Helpers.Net.fst
@@ -1,0 +1,34 @@
+(* BPFStar.Helpers.Net -- implementation.
+   All networking operations are axiomatised. *)
+module BPFStar.Helpers.Net
+
+open Pulse.Lib.Pervasives
+module A = Pulse.Lib.Array
+open FStar.Ghost
+open BPFStar.Types
+open BPFStar.ProgType
+open BPFStar.KPtr
+
+(* XDP *)
+let bpf_xdp_adjust_head #_ #_ _ _ = admit ()
+let bpf_xdp_adjust_tail #_ #_ _ _ = admit ()
+let bpf_xdp_adjust_meta #_ #_ _ _ = admit ()
+let bpf_redirect_map #_ #_ _ _ _ = admit ()
+
+(* TC *)
+let bpf_skb_store_bytes #_ #_ _ _ _ _ _ = admit ()
+let bpf_skb_change_proto #_ #_ _ _ _ = admit ()
+let bpf_skb_change_head #_ #_ _ _ _ = admit ()
+let bpf_skb_change_tail #_ #_ _ _ _ = admit ()
+let bpf_skb_pull_data #_ #_ _ _ = admit ()
+let bpf_skb_adjust_room #_ #_ _ _ _ _ = admit ()
+let bpf_l3_csum_replace #_ #_ _ _ _ _ _ = admit ()
+let bpf_l4_csum_replace #_ #_ _ _ _ _ _ = admit ()
+
+(* XDP + TC *)
+let bpf_redirect #_ #_ _ _ = admit ()
+let bpf_fib_lookup #_ #_ #_ _ _ _ _ = admit ()
+let bpf_csum_diff #_ #_ _ _ _ _ _ = admit ()
+
+(* TC + socket_filter *)
+let bpf_skb_load_bytes #_ #_ _ _ _ _ = admit ()
