lib/BPFStar.Helpers.Storage.fst
@@ -1,0 +1,29 @@
+(* BPFStar.Helpers.Storage -- implementation.
+   All storage operations are axiomatised. *)
+module BPFStar.Helpers.Storage
+
+open Pulse.Lib.Pervasives
+open FStar.Ghost
+open BPFStar.Types
+open BPFStar.ProgType
+open BPFStar.KPtr
+open BPFStar.Map
+
+let storage_perm #_ _ = emp
+let storage_value #_ _ _ _ = emp
+
+let release_storage_value #_ _ _ = admit ()
+let read_storage_value #_ _ _ = admit ()
+let write_storage_value #_ _ _ _ = admit ()
+
+let bpf_inode_storage_get #_ #_ #_ _ _ _ _ = admit ()
+let bpf_inode_storage_delete #_ #_ #_ _ _ = admit ()
+
+let bpf_task_storage_get #_ _ _ _ _ = admit ()
+let bpf_task_storage_delete #_ _ _ = admit ()
+
+let bpf_cgrp_storage_get #_ _ _ _ _ = admit ()
+let bpf_cgrp_storage_delete #_ _ _ = admit ()
+
+let bpf_sk_storage_get #_ #_ #_ _ _ _ _ = admit ()
+let bpf_sk_storage_delete #_ #_ #_ _ _ = admit ()
