lib/BPFStar.SpinLock.fst
@@ -1,0 +1,13 @@
+(* BPFStar.SpinLock -- implementation.
+   Lock operations are axiomatised. *)
+module BPFStar.SpinLock
+
+open Pulse.Lib.Pervasives
+open BPFStar.Types
+
+let bpf_spin_lock_t = unit
+
+let lock_inv _ _ = emp
+
+let bpf_spin_lock #_ _ = admit ()
+let bpf_spin_unlock #_ _ = admit ()
